fixed docstrings, eval uses eval\2 as reference

CompPoly/Univariate/Raw/Ops.lean
@@ -26,17 +26,18 @@ variable {S : Type*}
 
 /-- Evaluates a `CPolynomial.Raw` at `x : S` using a ring homomorphism `f : R →+* S`.
 
-  Computes `f(a₀) + f(a₁) * x + f(a₂) * x² + ...` where `aᵢ` are the coefficients.
-
-  TODO: define an efficient version of this with caching -/
+  Computes `f(a₀) + f(a₁) * x + f(a₂) * x² + ...` where `aᵢ` are the coefficients.  -/
 def eval₂ [Semiring R] [Semiring S] (f : R →+* S) (x : S) (p : CPolynomial.Raw R) : S :=
   p.zipIdx.foldl (fun acc ⟨a, i⟩ => acc + f a * x ^ i) 0
 
+@[inline, specialize]
 def eval₂Horner [Semiring R] [Semiring S] (f : R →+* S) (x : S) (p : CPolynomial.Raw R) : S :=
   p.foldr (fun a acc => acc * x + f a) 0
 
-lemma foldl_zipIdx_eq_foldr_pow_k [Semiring R] [Semiring S] (f : R →+* S) (x : S) (init : S) (k : Nat) (l : List R) :
-  List.foldl (fun acc a => acc + (f a.1) * x ^ a.2) init (l.zipIdx k) = List.foldr (fun a acc => acc * x + f a) 0 l * x ^ k + init := by
+private lemma foldl_zipIdx_eq_foldr_pow_k [Semiring R] [Semiring S]
+    (f : R →+* S) (x : S) (init : S) (k : Nat) (l : List R) :
+    List.foldl (fun acc a => acc + (f a.1) * x ^ a.2) init (l.zipIdx k) =
+      List.foldr (fun a acc => acc * x + f a) 0 l * x ^ k + init := by
     induction l generalizing init k with
     | nil => simp
     | cons head tail tail_ih =>
@@ -44,8 +45,9 @@ lemma foldl_zipIdx_eq_foldr_pow_k [Semiring R] [Semiring S] (f : R →+* S) (x :
            rw [tail_ih]
            rw [add_mul, mul_assoc, ← pow_succ', add_comm init, add_assoc]
 
-theorem eval₂_eq_eval₂Horner [Semiring R] [Semiring S] (f : R →+* S) (x : S) (p : CPolynomial.Raw R) :
-  eval₂ f x p = eval₂Horner f x p := by
+theorem eval₂_eq_eval₂Horner [Semiring R] [Semiring S]
+    (f : R →+* S) (x : S) (p : CPolynomial.Raw R) :
+    eval₂ f x p = eval₂Horner f x p := by
     unfold eval₂ eval₂Horner
     rw [← Array.foldl_toList, ← Array.foldr_toList, Array.toList_zipIdx]
     have := foldl_zipIdx_eq_foldr_pow_k f x 0 0 p.toList
@@ -54,7 +56,7 @@ theorem eval₂_eq_eval₂Horner [Semiring R] [Semiring S] (f : R →+* S) (x : 
 /-- Evaluates a `CPolynomial.Raw` at a given value -/
 @[inline, specialize]
 def eval [Semiring R] (x : R) (p : CPolynomial.Raw R) : R :=
-  p.eval₂Horner (RingHom.id R) x
+  p.eval₂ (RingHom.id R) x
 
 /-- Raw addition: pointwise sum of coefficient arrays (padded to equal length).
 
